isabelle/Auction/Sandbox/DynamicAuctionCodeExtraction.thy
@@ -7,11 +7,61 @@ Trust2
 
 begin
 
+
+
 definition "evaluateMe (input(*::(integer list => integer list)*)) 
 (output(*::(_ => integer list)*))
 = snd (output (String.implode ''Starting\<newline>Input the number of bidders:'', [])
 , dynamicAuction input output)"
 term evaluateMe
+
+definition "evaluateMe2 
+(input :: _)
+(output:: _) 
+= snd (output (
+String.implode ''Starting\<newline>Input the number of bidders:'', True, []),
+dynamicAuction input output)"
+ 
+
+(* 
+input and output will be the only manually written Scala functions 
+(and will be passed as arguments to evaluateMe as the only action of the main method of our Scala wrapper ) 
+- input will take a list as an argument, and grow it by the input (side effect) provided by the user.
+- output will take a pair (list, messageAfterEachBid) as an argument, will return list without touching it, 
+while printing messageAfterEachBid to the user (side effect).
+Thus, iterating the combined function output o XXX o input (where XXX is the Isabelle function doing 
+the ``real work''), evaluateMe will provide a dynamic auction execution.
+The length of the list passed to XXX will be used to determine in which round we are.
+
+Thus, the manually-written Scala code (to be appended to the Isabelle-generated lines) will be:
+*)
+
+(*
+def untrustedInput(n:List[String]) : List[String] = {
+	val x=readLine;
+	return (x::n);
+}
+
+def untrustedOutput(x: (List[String], String)) : List[String] = {
+	println(snd (x));
+	return (fst (x));
+}
+
+def main(args: Array[String]) {
+	val x=evaluateMe(untrustedInput, untrustedOutput);
+}
+
+*)
+
+(*
+It can't probably get thinner than this.
+My ambition would be to handle everything besides input/output from inside Isabelle, including
+conversion from strings (as from input) to numbers and viceversa (for output); 
+this is definitely possible, but how realistic given our schedule?
+We could momentarily choose to directly use Scala integers as input/output, 
+which is less robust/flexible/elegant but simpler.
+*)
+
 
 export_code fst snd evaluateMe evaluateMe2 in Scala module_name a file "/dev/shm/a.scala"
 end
